Some progress
I think I need to rewrite my environment

src/Base.thy
@@ -4,69 +4,135 @@ imports Main
 
 begin
 
-definition
-  shift :: "(nat \<Rightarrow> 'a) \<Rightarrow> nat \<Rightarrow> 'a \<Rightarrow> nat \<Rightarrow> 'a"  ("_, _:_" [90, 0, 0] 91) where
-  "\<Gamma>, i:a = (\<lambda>j. if j < i then \<Gamma> j else if j = i then a else \<Gamma> (j - 1))"
-
-text \<open>
-lemma shift_eq [simp]: "i = j \<Longrightarrow> (\<Gamma>, i:T) j = T"
-  by (simp add: shift_def)
-
-lemma shift_gt [simp]: "j < i \<Longrightarrow> (\<Gamma>, i:T) j = \<Gamma> j"
-  by (simp add: shift_def)
-
-lemma shift_lt [simp]: "i < j \<Longrightarrow> (\<Gamma>, i:T) j = \<Gamma> (j - 1)"
-  by (simp add: shift_def)
-
-lemma shift_commute [simp]: "\<Gamma>, i:U, 0:T = \<Gamma>, 0:T, Suc i:U"
-  by (rule ext) (simp_all add: shift_def split: nat.split)
-\<close>
-
 type_synonym varName = nat
 type_synonym typeName = nat
 
 datatype "type" =
 	Atom typeName
-	| Fun type type (infixr "->" 200)
+	| Arrow type type (infixr "->" 200)
+	| Unit
 
 type_synonym varCtx = "varName => type"
 
 
 datatype "term" =
-	Var "varName"
-	| Abs varName "type" "term"
-	| App "term" "term" (infixl "\<degree>" 200)
+      var "varName"
+      | abs varName "type" "term"
+      | app "term" "term"
+      | unit
 
-inductive "value" :: "term => bool" where
-	"value (Abstraction _ _ _)"
+
+definition
+  shift :: "(varName \<Rightarrow> 'a) \<Rightarrow> varName \<Rightarrow> 'a \<Rightarrow> varName \<Rightarrow> 'a"  ("_, <_:_>" [90, 0, 0] 91) where
+  "\<Gamma>, <i:a> = (\<lambda>j. if j < i then \<Gamma> j else if j = i then a else \<Gamma> (j - 1))"
+
+lemma shift_eq [simp]: "i = j \<Longrightarrow> (\<Gamma>, <i:T>) j = T"
+  by (simp add: shift_def)
+
+lemma shift_gt [simp]: "j < i \<Longrightarrow> (\<Gamma>, <i:T>) j = \<Gamma> j"
+  by (simp add: shift_def)
+
+lemma shift_lt [simp]: "i < j \<Longrightarrow> (\<Gamma>, <i:T>) j = \<Gamma> (j - 1)"
+  by (simp add: shift_def)
+
+lemma shift_commute [simp]: "\<Gamma>, <i:U>, <0:T> = \<Gamma>, <0:T>, <Suc i:U>"
+  by (rule ext) (simp_all add: shift_def split: nat.split)
 
 primrec
-  substn :: "[term, term, nat] => term"
+  lift :: "[term, varName] => term"
 where
-    "substn (Var i) s k =
-      (if k < i then Var (i - 1) else if i = k then liftn k s 0 else Var i)"
-  | "substn (t ° u) s k = substn t s k ° substn u s k"
-  | "substn (Abs k T t) s k = Abs (substn t s (k + 1))"
+    "lift (var i) x = (if i < x then var i else var (i + 1))"
+  | "lift (app s t) x = app (lift s x) (lift t x)"
+  | "lift (abs x T s) y = abs x T (lift s (y + 1))"
+  | "lift unit x = unit"
 
-text \<open> TODO: Add value requirements\<close>
+primrec subst_term :: "[term, varName, term] => term" ("_[_ ~> _]" [300, 0, 0] 300)
+	where
+	subst_var: "(var x)[y ~> t] = (if x = y then t else if x < y then var x else var (x - 1))"
+	| subst_app: "(app t1 t2)[y ~> t] = app (t1[y ~> t]) (t2[y ~> t])"
+	| subst_abs: "(abs x T1 t1)[y ~> t] = abs x T1 (t1[y + 1 ~> lift t 0])"
+	| subst_unit: "unit[y ~> t] = unit"
+
+inductive "value" :: "term => bool"
+  where
+      val_abs: "value (abs _ _ _)"
+      | val_unit: "value unit"
+
+(*
+primrec liftn :: "[nat, term, nat] => term"
+  where
+    "liftn n (var i) k = (if i < k then var i else var (i + n))"
+  | "liftn n (app s t) k = app (liftn n s k) (liftn n t k)"
+  | "liftn n (abs x T s) k = abs x T (liftn n s (k + 1))"
+  | "liftn n unit k = unit"
+
+primrec substn :: "[term, term, nat] => term"
+  where
+    "substn (var i) s k =
+      (if k < i then var (i - 1) else if i = k then liftn k s 0 else var i)"
+  | "substn (app t u) s k = app (substn t s k) (substn u s k)"
+  | "substn (abs x T t) s k = substn t s (k + 1)"
+  | "substn unit s k = unit"
+*)
+
 inductive "evaluation" :: "[term, term] \<Rightarrow> bool" (infixl "\<rightarrow>" 50)
   where
-    e_app_1: "t1 \<rightarrow> t1' \<Longrightarrow> t1 \<degree> t2 \<rightarrow> t1' \<degree> t2"
-    e_app_2: "t2 \<rightarrow> t2' \<Longrightarrow> t1 \<degree> t2 \<rightarrow> t1 \<degree> t2'"
-    e_app_abs: "Abs x T t"
+    e_app_1: "t1 \<rightarrow> t1' \<Longrightarrow> app t1 t2 \<rightarrow> app t1' t2"
+  | e_app_2: "t2 \<rightarrow> t2' \<Longrightarrow> app t1 t2 \<rightarrow> app t1 t2'"
+  | e_app_abs: "value t2 \<Longrightarrow> app (abs x T t) t2 \<rightarrow> (substn t t2 x)"
 
 
-inductive
-	typing :: "varCtx => term => type => bool" ("_ ⊢ _ : _" [50, 50, 50] 50)
-
-	where
-
-	t_abs : "\<Gamma>, x:T1 ⊢ t2 : T2 ==> \<Gamma> ⊢ Abs x T1 t : (T1 -> T2)"
-	| t_var : "\<Gamma>(x) = T ==> \<Gamma> ⊢ (Var x) : T"
-	| t_app : "\<Gamma> ⊢ t1 : (T1 -> T2) ==> \<Gamma> ⊢ t2 : T1 ==> \<Gamma>  ⊢ (t1 \<degree> t2) : T2"
+inductive typing :: "varCtx => term => type => bool" ("_ ⊢ _ : _" [50, 50, 50] 50)
+  where
+    t_abs [intro!]: "\<Gamma>, <x:T1> ⊢ t2 : T2 ==> \<Gamma> ⊢ abs x T1 t2 : (T1 -> T2)"
+  | t_var [intro!]: "\<Gamma>(x) = T ==> \<Gamma> ⊢ var x : T"
+  | t_app [intro!]: "\<Gamma> ⊢ t1 : (T1 -> T2) ==> \<Gamma> ⊢ t2 : T1 ==> \<Gamma>  ⊢ app t1 t2 : T2"
+  | t_unit [intro!]: "\<Gamma> ⊢ unit : Unit"
 
 inductive_cases typing_elims [elim!]:
-  "\<Gamma> ⊢ Var x : T"
-  "\<Gamma> ⊢ t \<degree> u : T"
-  "\<Gamma> ⊢ Abs x T1 t : T"
+  "\<Gamma> ⊢ var x : T"
+  "\<Gamma> ⊢ app t u : T"
+  "\<Gamma> ⊢ abs x T1 t : T"
+  "\<Gamma> ⊢ unit : Unit"
 
+schematic_goal "\<Gamma> ⊢ app (abs x Unit (var x)) unit : ?T"
+	by force
+
+lemma subst_eq [simp]: "(var x)[x ~> t] = t"
+  by (simp add: subst_var)
+
+lemma subst_gt [simp]: "y < x ==> (var x)[y ~> t] = var (x - 1)"
+  by (simp add: subst_var)
+
+lemma subst_lt [simp]: "y > x ==> (var x)[y ~> t] = var x"
+  by (simp add: subst_var)
+
+lemma canonical_forms_abs:
+  fixes t :: "term"
+	assumes d: "\<Gamma> ⊢ t : (T1 -> T2)"
+		and v: "value t"
+	shows "∃ x T1 t2 .t = abs x T1 t2"
+  using d typing.cases v value.simps by blast
+
+lemma canonical_forms_unit:
+	fixes t :: "term"
+	assumes d: "\<Gamma> ⊢ t : Unit"
+	  and v: "value t"
+	shows "t = unit" using d v value.simps by auto
+
+theorem progress:
+	assumes d: "\<Gamma> ⊢ t : T"
+	shows "(value t) | (t \<rightarrow> t')"
+	sorry
+
+lemma subst_lemma:
+	assumes d1: "\<Gamma>, <x:T2> ⊢ t1 : T1"
+		and d2: "\<Gamma> ⊢ t2 : T2"
+	shows "\<Gamma> ⊢ t1[x ~> t2] : T1"
+	sorry
+
+theorem preservation:
+	assumes d: "\<Gamma> ⊢ t : T"
+		and e: "t \<rightarrow> t'"
+	shows "\<Gamma> ⊢ t' : T"
+	sorry
